Update borrowing machinery with merger

nola/iris/borrow.v
@@ -3,60 +3,58 @@
 From nola.util Require Export prod.
 From nola.iris Require Import util.
 From nola.iris Require Export lft upd.
+From nola.util Require Import prod.
 From iris.algebra Require Import numbers excl agree gmap auth.
 From iris.bi Require Import fractional.
 From iris.base_logic.lib Require Import ghost_map.
 From iris.proofmode Require Import proofmode.
 
+(** ** Ghost state *)
+
 Implicit Type PROP : Type.
 Implicit Type (α : lft) (q : Qp).
 
-(** ** Ghost state *)
-
-(** Algebra for the depth bounding *)
-Definition depthR := authR max_natR.
-Implicit Type d g : nat.
-
-(** ID for a borrower/lender *)
+(** ID for a borrower/deposit/lender *)
 Local Definition bor_id := positive.
+Local Definition depo_id := positive.
 Local Definition lend_id := positive.
-Implicit Type (j : bor_id) (i : lend_id).
+Implicit Type (i : depo_id) (j : bor_id) (k : lend_id).
 
-(** Kind of a borrower *)
-Variant bor_kind :=
+(** Mode of a borrower *)
+Variant bor_mode : Set :=
 | #[local] Clsd (* Closed *)
 | #[local] Open (q : Qp) (* Open with a fraction *)
 | #[local] Rebor (α : lft) (* Reborrowed *).
-Implicit Type b : bor_kind.
+Implicit Type b : bor_mode.
 (** State of a borrower *)
-Local Definition bor_st PROP : Type :=
-  PROP *' bor_kind (* Deposited fraction *).
+Local Definition bor_st PROP : Type := PROP *' bor_mode.
 (** State of the borrowers *)
-Local Definition bor_stm PROP : Type := gmap bor_id (bor_st PROP).
+Local Notation bor_stm PROP := (gmap bor_id (bor_st PROP)).
 
-(** Kind of a lender *)
-Variant lend_kind :=
-| #[local] Lend (* Lending *)
-| #[local] Dead (* Dead *).
-Implicit Type l : lend_kind.
-(** Core state of a lender *)
-Local Definition lend_cst PROP : Type := nat (* Depth *) *' PROP *' lend_kind.
-(** State of a lender *)
-Local Definition lend_st PROP : Type :=
-  lft *' lend_cst PROP *' bor_stm PROP.
 (** State of the lenders *)
-Local Definition lend_stm PROP : Type := gmap lend_id (lend_st PROP).
+Local Notation lendm PROP := (gmap lend_id PROP).
+
+(** Kind of a deposit *)
+Local Definition depo_kind : Type := nat (* depth *) *' lft.
+Implicit Type e : depo_kind.
+(** State of a deposit *)
+Local Definition depo_st PROP : Type :=
+  depo_kind *' bor_stm PROP *' lendm PROP.
+(** State of the deposits *)
+Local Notation depo_stm PROP := (gmap depo_id (depo_st PROP)).
 
 (** Algebra for a borrower *)
 Local Definition borR PROP := exclR (leibnizO (bor_st PROP)).
-
 (** Algebra for a lender *)
-Local Definition lendR PROP := prodR
-  (prodR (agreeR (leibnizO lft)) (optionR (exclR (leibnizO (lend_cst PROP)))))
-  (gmapR bor_id (borR PROP)).
+Local Definition lendR PROP := exclR (leibnizO PROP).
+(** Algebra for a deposit *)
+Local Definition depoR PROP := prodR (prodR
+  (agreeR (leibnizO depo_kind))
+  (gmapR bor_id (borR PROP)))
+  (gmapR lend_id (lendR PROP)).
 
 (** Algebra for the borrowing machinery *)
-Local Definition borrowR_def PROP := authR (gmapR lend_id (lendR PROP)).
+Local Definition borrowR_def PROP := authR (gmapR depo_id (depoR PROP)).
 Local Lemma borrowR_aux : seal borrowR_def. Proof. by eexists. Qed.
 Definition borrowR := borrowR_aux.(unseal).
 Local Lemma borrowR_unseal : borrowR = borrowR_def.
@@ -65,22 +63,19 @@ Proof. exact: borrowR_aux.(seal_eq). Qed.
 (** Ghost state for the borrowing machinery *)
 Class borrowGS PROP Σ := BorrowGS {
   borrowGS_lft :: lftG Σ;
-  borrowGS_depth :: inG Σ depthR;
   borrowGS_borrow :: inG Σ (borrowR PROP);
-  depth_name : gname; borrow_name : gname;
+  borrow_name : gname;
 }.
-Local Existing Instance borrowGS_depth.
 Local Existing Instance borrowGS_borrow.
 Local Instance inG_borrow_def `{!inG Σ (borrowR PROP)} :
   inG Σ (borrowR_def PROP).
-Proof. rewrite -borrowR_unseal. apply _. Qed.
+Proof. rewrite -borrowR_unseal. exact _. Qed.
 Class borrowGpreS PROP Σ := BorrowGpreS {
   borrowGpreS_lft :: lftG Σ;
-  borrowGpreS_depth :: inG Σ depthR;
   borrowGpreS_borrow :: inG Σ (borrowR PROP);
 }.
 Definition borrowΣ PROP : gFunctors :=
-  #[GFunctor lftR; GFunctor depthR; GFunctor (borrowR PROP)].
+  #[GFunctor lftR; GFunctor (borrowR PROP)].
 #[export] Instance subG_borrow `{!subG (borrowΣ PROP) Σ} : borrowGpreS PROP Σ.
 Proof. solve_inG. Qed.
 
@@ -88,49 +83,32 @@ Proof. solve_inG. Qed.
 
 Section borrow.
   Context `{!borrowGS PROP Σ}.
-  Implicit Type (P Q : PROP)
-    (B : bor_st PROP) (L : lend_st PROP) (Lm : lend_stm PROP).
-
-  (** Witness of a depth *)
-  Local Definition depth d : iProp Σ := own depth_name (◯ (MaxNat d)).
-  (** Global bound of the depths *)
-  Local Definition gdepth g : iProp Σ := own depth_name (● (MaxNat g)).
-
-  (** Get [depth 0] *)
-  Local Lemma depth_0 : ⊢ |==> depth 0. Proof. apply own_unit. Qed.
-  (** Introduce a new depth *)
-  Local Lemma depth_alloc {g d} : gdepth g ==∗ ∃ g', gdepth g' ∗ depth d.
-  Proof.
-    iIntros "g". iMod (own_update with "g") as "[? $]"; [|by iExists _].
-    apply auth_update_alloc, local_update_unital_discrete=> ? _.
-    by rewrite left_id=> <-.
-  Qed.
-
-  (** Bounding by [gdepth] *)
-  Local Lemma depth_bound {g d} : gdepth g -∗ depth d -∗ ⌜d ≤ g⌝.
-  Proof.
-    iIntros "g d". iDestruct (own_valid_2 with "g d") as %v. iPureIntro.
-    by move: v=> /auth_both_valid_discrete [/max_nat_included ? _].
-  Qed.
+  Implicit Type (P Q : PROP) (Pl Ql : list PROP)
+    (D : depo_st PROP) (Dm : depo_stm PROP)
+    (B : bor_st PROP) (Bm : bor_stm PROP) (Pm : lendm PROP).
 
   (** General borrower token *)
-  Local Definition bor_itok i j α B : iProp Σ :=
-    own borrow_name (◯ {[i := (to_agree α, ε, {[j := Excl B]})]}).
+  Local Definition bor_itok i j d α B : iProp Σ :=
+    own borrow_name (◯ {[i := (to_agree (d, α)', {[j := Excl B]}, ε)]}).
 
-  (** Closed borrower token *)
+  (** Closed borrower token
+
+    It may be a dead lifetime token or a closed borrower
+
+    Slightly stronger than [bor_tok] *)
   Local Definition bor_ctok_def α P : iProp Σ :=
-    [†α] ∨ ∃ α', α ⊑s α' ∗ (∃ i j, bor_itok i j α' (P, Clsd)').
+    [†α] ∨ ∃ i j d α', α ⊑□ α' ∗ bor_itok i j d α' (P, Clsd)'.
   Local Lemma bor_ctok_aux : seal bor_ctok_def. Proof. by eexists. Qed.
   Definition bor_ctok := bor_ctok_aux.(unseal).
   Local Lemma bor_ctok_unseal : bor_ctok = bor_ctok_def.
   Proof. exact: bor_ctok_aux.(seal_eq). Qed.
+
   (** Borrower token
 
-    It may be a dead lifetime token, a closed borrower,
-    or an retrieving reborrower *)
+    It may be [bor_tok] or a retrieving reborrower *)
   Local Definition bor_tok_def α P : iProp Σ :=
-    bor_ctok α P ∨
-    ∃ α', α ⊑s α' ∗ ∃ i j β, [†β] ∗ bor_itok i j α' (P, Rebor β)'.
+    bor_ctok α P ∨ ∃ i j d α' β,
+      α ⊑□ α' ∗ [†β] ∗ bor_itok i j d α' (P, Rebor β)'.
   Local Lemma bor_tok_aux : seal bor_tok_def. Proof. by eexists. Qed.
   Definition bor_tok := bor_tok_aux.(unseal).
   Local Lemma bor_tok_unseal : bor_tok = bor_tok_def.
@@ -138,243 +116,279 @@ Section borrow.
 
   (** Open borrower token
 
-    It keeps a lifetime token at hand *)
+    It keeps a lifetime token [(r/2).[α']] at hand *)
   Local Definition bor_otok_def α P q : iProp Σ :=
-    ∃ α' r, α ⊑s α' ∗ (r.[α'] -∗ q.[α]) ∗
-      (r/2).[α'] ∗ ∃ i j, bor_itok i j α' (P, Open (r/2))'.
+    ∃ α' r i j d, α ⊑□ α' ∗ (r.[α'] -∗ q.[α]) ∗
+      (r/2).[α'] ∗ bor_itok i j d α' (P, Open (r/2))'.
   Local Lemma bor_otok_aux : seal bor_otok_def. Proof. by eexists. Qed.
   Definition bor_otok := bor_otok_aux.(unseal).
   Local Lemma bor_otok_unseal : bor_otok = bor_otok_def.
   Proof. exact: bor_otok_aux.(seal_eq). Qed.
 
   (** Lender token *)
-  Local Definition lend_itok i α d P : iProp Σ :=
-    own borrow_name (◯ {[i := (to_agree α, Excl' (d, P, Lend)', ε)]}).
-  Local Definition lend_dtok α d P : iProp Σ :=
-    depth d ∗ ∃ i, lend_itok i α d P.
+  Local Definition lend_itok i k d α P : iProp Σ :=
+    own borrow_name (◯ {[i := (to_agree (d, α)', ε, {[k := Excl P]})]}).
+  Local Definition lend_dtok d α P : iProp Σ :=
+    ∃ i k, lend_itok i k d α P.
   Local Definition lend_tok_def α P : iProp Σ :=
-    ∃ α', α' ⊑s α ∗ ∃ d, lend_dtok α' d P.
+    ∃ α', α' ⊑□ α ∗ ∃ d, lend_dtok d α' P.
   Local Lemma lend_tok_aux : seal lend_tok_def. Proof. by eexists. Qed.
   Definition lend_tok := lend_tok_aux.(unseal).
   Local Lemma lend_tok_unseal : lend_tok = lend_tok_def.
   Proof. exact: lend_tok_aux.(seal_eq). Qed.
 
-  (** Convert a closed borrower token into a borrower token *)
+  (** Borrower and lender tokens are timelesss *)
+  #[export] Instance bor_ctok_timeless {α P} : Timeless (bor_ctok α P).
+  Proof. rewrite bor_ctok_unseal. apply _. Qed.
+  #[export] Instance bor_tok_timeless {α P} : Timeless (bor_tok α P).
+  Proof. rewrite bor_tok_unseal. apply _. Qed.
+  #[export] Instance bor_otok_timeless {α P q} : Timeless (bor_otok α P q).
+  Proof. rewrite bor_otok_unseal. apply _. Qed.
+  #[export] Instance lend_tok_timeless {α P} : Timeless (lend_tok α P).
+  Proof. rewrite lend_tok_unseal. apply _. Qed.
+
+  (** Turn [bor_ctok] to [bor_tok] *)
   Lemma bor_ctok_tok {α P} : bor_ctok α P ⊢ bor_tok α P.
   Proof. rewrite bor_tok_unseal. iIntros. by iLeft. Qed.
-  (** Fake a closed borrower from the dead lifetime token *)
+
+  (** Fake a borrower token from the dead lifetime token *)
   Lemma bor_ctok_fake {α P} : [†α] ⊢ bor_ctok α P.
   Proof. rewrite bor_ctok_unseal. iIntros. by iLeft. Qed.
-  (** Fake a borrower from the dead lifetime token *)
   Lemma bor_tok_fake {α P} : [†α] ⊢ bor_tok α P.
   Proof. by rewrite bor_ctok_fake bor_ctok_tok. Qed.
 
   (** Modify the lifetime of borrower and lender tokens *)
-  Lemma bor_ctok_lft {α α' P} : α' ⊑s α -∗ bor_ctok α P -∗ bor_ctok α' P.
+  Lemma bor_ctok_lft {α α' P} : α' ⊑□ α -∗ bor_ctok α P -∗ bor_ctok α' P.
   Proof.
-    rewrite bor_ctok_unseal. iIntros "#? [#?|[%α''[? c]]]".
-    { iLeft. by iApply lft_sincl_dead_acc. }
-    iRight. iExists _. iFrame "c". by iApply lft_sincl_trans.
+    rewrite bor_ctok_unseal. iIntros "#? [?|c]".
+    { iLeft. by iApply lft_sincl_dead. }
+    iDestruct "c" as (????) "[#? c]". iRight. iExists _, _, _, _. iFrame "c".
+    by iApply lft_sincl_trans.
   Qed.
-  Lemma bor_tok_lft {α α' P} : α' ⊑s α -∗ bor_tok α P -∗ bor_tok α' P.
-    rewrite bor_tok_unseal. iIntros "#? [c|[%α''[#? r]]]".
-    { iLeft. by iApply bor_ctok_lft. }
-    iRight. iExists _. iFrame "r". by iApply lft_sincl_trans.
+  #[export] Instance bor_ctok_mono : Proper (flip (⊑) ==> (=) ==> (⊢)) bor_ctok.
+  Proof. move=>/= ?????<-. iApply bor_ctok_lft. by iApply lft_incl_sincl. Qed.
+  #[export] Instance bor_ctok_mono' :
+    Proper ((⊑) ==> (=) ==> flip (⊢)) bor_ctok.
+  Proof. solve_proper. Qed.
+  Lemma bor_tok_lft {α α' P} : α' ⊑□ α -∗ bor_tok α P -∗ bor_tok α' P.
+  Proof.
+    rewrite bor_tok_unseal. iIntros "#⊑ [c|r]".
+    { iLeft. by iApply (bor_ctok_lft with "⊑ c"). }
+    iDestruct "r" as (?????) "[#? r]". iRight. iExists _, _, _, _, _.
+    iFrame "r". by iApply lft_sincl_trans.
   Qed.
+  #[export] Instance bor_tok_mono : Proper (flip (⊑) ==> (=) ==> (⊢)) bor_tok.
+  Proof. move=>/= ?????<-. iApply bor_tok_lft. by iApply lft_incl_sincl. Qed.
+  #[export] Instance bor_tok_mono' : Proper ((⊑) ==> (=) ==> flip (⊢)) bor_tok.
+  Proof. solve_proper. Qed.
   Lemma bor_otok_lft {α α' P q r} :
-    α' ⊑s α -∗ (q.[α] -∗ r.[α']) -∗ bor_otok α P q -∗ bor_otok α' P r.
+    α' ⊑□ α -∗ (q.[α] -∗ r.[α']) -∗ bor_otok α P q -∗ bor_otok α' P r.
   Proof.
-    rewrite bor_otok_unseal. iIntros "#? →α' [%α''[%s[#?[→α o]]]]".
-    iExists _, _. iFrame "o". iSplit; [by iApply lft_sincl_trans|].
-    iIntros "α''". iApply "→α'". by iApply "→α".
+    rewrite bor_otok_unseal. iIntros "#? →α'".
+    iDestruct 1 as (α'' ????) "[#?[→α o]]". iExists _, _, _, _, _. iFrame "o".
+    iSplit; [by iApply lft_sincl_trans|]. iIntros "α''". iApply "→α'".
+    by iApply "→α".
   Qed.
-  Lemma lend_tok_lft {α α' P} : α ⊑s α' -∗ lend_tok α P -∗ lend_tok α' P.
+  Lemma lend_tok_lft {α α' P} : α ⊑□ α' -∗ lend_tok α P -∗ lend_tok α' P.
   Proof.
     rewrite lend_tok_unseal. iIntros "#? [%α''[#? l]]". iExists _. iFrame "l".
     by iApply lft_sincl_trans.
   Qed.
+  #[export] Instance lend_tok_mono : Proper ((⊑) ==> (=) ==> (⊢)) lend_tok.
+  Proof. move=>/= ?????<-. iApply lend_tok_lft. by iApply lft_incl_sincl. Qed.
+  #[export] Instance lend_tok_mono' :
+    Proper (flip (⊑) ==> (=) ==> flip (⊢)) lend_tok.
+  Proof. solve_proper. Qed.
 
-  (** Token for [lend_stm] *)
-  Local Definition lend_st_to_lendR L : lendR PROP :=
-    let '(α, C, Bm)' := L in
-    (to_agree α, Excl' C, (Excl : bor_st _ → _) <$> Bm).
-  Local Definition lend_stm_tok Lm : iProp Σ :=
-    own borrow_name (● (lend_st_to_lendR <$> Lm : gmapR _ _)).
+  (** Token for [depo_stm] *)
+  Local Definition depo_st_R D : depoR PROP :=
+    let '(e, Bm, Pm)' := D in (to_agree e, Excl <$> Bm, Excl <$> Pm).
+  Arguments depo_st_R _ /.
+  Local Definition depo_stm_tok Dm : iProp Σ :=
+    own borrow_name (● (depo_st_R <$> Dm : gmapR _ _)).
 
-  (** Create [bor_itok] and [lend_itok] w.r.t. [lend_stm_tok] *)
-  Local Lemma lend_stm_create {Lm} d α P :
-    lend_stm_tok Lm -∗ |==> ∃ i j,
-      lend_stm_tok (<[i := (α, (d, P, Lend)', {[j := (P, Clsd)']})']> Lm) ∗
-      bor_itok i j α (P, Clsd)' ∗ lend_itok i α d P.
+  (** Lemma for [to_bor_itoks] *)
+  Local Lemma bor_insert_op {i j e B Bm} :
+    Bm !! j = None →
+    (◯ {[i := (to_agree e, Excl <$> <[j:=B]> Bm, ε)]} : borrowR_def _) ≡
+      ◯ {[i := (to_agree e, {[j:=Excl B]}, ε)]} ⋅
+      ◯ {[i := (to_agree e, Excl <$> Bm, ε)]}.
   Proof.
-    iIntros "●". iExists (fresh (dom Lm)), 1%positive.
-    iMod (own_update with "●") as "[$[$$]]"; [|done].
-    rewrite -auth_frag_op singleton_op fmap_insert. apply auth_update_alloc.
-    have <- :
-      lend_st_to_lendR (α, (d, P, Lend)', {[1%positive := (P, Clsd)']})' ≡
-      ((to_agree α, ε, {[1%positive := Excl (P, Clsd)']}) : lendR _) ⋅
-        (to_agree α, Excl' (d, P, Lend)', ε).
-    { split; [split|]=>/=; by [rewrite agree_idemp|]. }
-    apply alloc_singleton_local_update.
-    - rewrite lookup_fmap. apply fmap_None, not_elem_of_dom_1, is_fresh.
-    - split; [split|]=>/=; by [|rewrite map_fmap_singleton singleton_valid].
+    move=> eq. rewrite fmap_insert -auth_frag_op. f_equiv. rewrite singleton_op.
+    apply: singletonM_proper.
+    split; [split|]=>/=; [by rewrite agree_idemp| |done].
+    rewrite (insert_singleton_op _ _ (_ : borR _)); [done|].
+    rewrite lookup_fmap. by rewrite eq.
+  Qed.
+  (** Get [bor_itok]s out of [own] *)
+  Local Lemma to_bor_itoks {i d α Bm} :
+    own borrow_name (◯ {[i := (to_agree (d, α)', Excl <$> Bm, ε)]}) ⊢
+      [∗ map] j ↦ B ∈ Bm, bor_itok i j d α B.
+  Proof.
+    induction Bm as [|j B Bm ? IH] using map_ind.
+    { rewrite big_sepM_empty. by iIntros. }
+    rewrite big_sepM_insert; [|done]. rewrite -IH bor_insert_op; [|done].
+    iIntros "[$$]".
   Qed.
 
-  (** Agreement between [lend_stm_tok] and [lend_itok] *)
-  Local Lemma lend_stm_lend_agree {Lm i α d P} :
-    lend_stm_tok Lm -∗ lend_itok i α d P -∗
-      ⌜∃ Bm, Lm !! i = Some (α, (d, P, Lend)', Bm)'⌝.
+  (** Lemma for [to_lend_itoks] *)
+  Local Lemma lend_insert_op {i k e P Pm} :
+    Pm !! k = None →
+    (◯ {[i := (to_agree e, ε, Excl <$> <[k:=P]> Pm)]} : borrowR_def _) ≡
+      ◯ {[i := (to_agree e, ε, {[k:=Excl P]})]} ⋅
+      ◯ {[i := (to_agree e, ε, Excl <$> Pm)]}.
+    move=> eq. rewrite fmap_insert -auth_frag_op. f_equiv. rewrite singleton_op.
+    apply: singletonM_proper.
+    split; [split|]=>/=; [by rewrite agree_idemp|done|].
+    rewrite (insert_singleton_op _ _ (_ : exclR (leibnizO _))); [done|].
+    rewrite lookup_fmap. by rewrite eq.
+  Qed.
+  (** Get [lend_itok]s out of [own] *)
+  Local Lemma to_lend_itoks {i d α Pm} :
+    own borrow_name (◯ {[i := (to_agree (d, α)', ε, Excl <$> Pm)]}) ⊢
+      [∗ map] k ↦ P ∈ Pm, lend_itok i k d α P.
+  Proof.
+    induction Pm as [|k P Pm ? IH] using map_ind.
+    { rewrite big_sepM_empty. by iIntros. }
+    rewrite big_sepM_insert; [|done]. rewrite -IH lend_insert_op; [|done].
+    iIntros "[$$]".
+  Qed.
+
+  (** Create [bor_itok]s and [lend_itok]s w.r.t. [depo_stm_tok] *)
+  Local Lemma depo_stm_bor_lend_new {Dm} d α Pl Ql :
+    depo_stm_tok Dm -∗ |==> ∃ i,
+      let Bm := map_by _ (fmap (M:=list) (λ P, (P, Clsd)') Pl) in
+      let Qm := map_by _ Ql in
+      depo_stm_tok (<[i := ((d, α)', Bm, Qm)']> Dm) ∗
+      ([∗ map] j ↦ B ∈ Bm, bor_itok i j d α B) ∗
+      [∗ map] k ↦ Q ∈ Qm, lend_itok i k d α Q.
+  Proof.
+    iIntros "●". iExists (fresh (dom Dm)).
+    iMod (own_update with "●") as "[$[c l]]"; last first.
+    { iModIntro. iDestruct (to_bor_itoks (d:=d) with "c") as "$".
+      iApply (to_lend_itoks with "l"). }
+    rewrite -auth_frag_op singleton_op fmap_insert.
+    have <- : ∀ x y, ((to_agree (d, α)', x, y) : depoR _) ≡
+      ((to_agree (d, α)', x, ε) : depoR _) ⋅ (to_agree (d, α)', ε, y).
+    { split; [split|]=>/=; by
+        [rewrite agree_idemp|rewrite left_id|rewrite right_id]. }
+    apply auth_update_alloc, alloc_singleton_local_update.
+    - rewrite lookup_fmap. apply fmap_None, not_elem_of_dom_1, is_fresh.
+    - split; [split|]=>/=; [done|by apply: gmap_fmap_valid..].
+  Qed.
+
+  (** Agreement between [depo_stm_tok] and [lend_itok] *)
+  Local Lemma depo_stm_lend_agree {Dm i k d α P} :
+    depo_stm_tok Dm -∗ lend_itok i k d α P -∗
+      ⌜∃ Bm Pm, Dm !! i = Some ((d, α)', Bm, Pm)' ∧ Pm !! k = Some P⌝.
   Proof.
     iIntros "● l". iDestruct (own_valid_2 with "● l") as %v. iPureIntro.
-    move: v=> /auth_both_valid_discrete[/singleton_included_l[?[
-      /Some_equiv_eq[[[??]?][/lookup_fmap_Some[[?[? Bm]][[<-<-<-]?]<-]]]
-      /Some_included_total/prod_included[/prod_included/=[
-        /to_agree_included/leibniz_equiv_iff?
-        /Excl_included/leibniz_equiv_iff?]_]]]_].
-    subst. by eexists _.
+    move: v=> /auth_both_valid_discrete[/singleton_included_l[?[++]]_].
+    move=> /Some_equiv_eq[[[??]?][+<-]].
+    move=> /lookup_fmap_Some[[?[??]][[<-<-<-]?]].
+    move=> /Some_included_total/prod_included[/prod_included/=[+_]inc].
+    move=> /to_agree_included/leibniz_equiv_iff ?.
+    apply singleton_included_exclusive_l in inc;
+      [|exact _|by apply: gmap_fmap_valid]. move: inc.
+    rewrite lookup_fmap leibniz_equiv_iff fmap_Some. move=> [?[?[?]]]. subst.
+    by eexists _, _.
   Qed.
-  (** Extend a lender w.r.t. [lend_stm_tok] *)
-  Local Lemma lend_stm_lend_extend {Lm i α d P Bm Q} :
-    Lm !! i = Some (α, (d, P, Lend)', Bm)' →
-    lend_stm_tok Lm -∗ lend_itok i α d P ==∗
-      lend_stm_tok (<[i := (α, (d, Q, Lend)', Bm)']> Lm) ∗ lend_itok i α d Q.
+  (** Delete a lender w.r.t. [depo_stm_tok] *)
+  Local Lemma depo_stm_lend_delete {Dm i k d α Bm Pm P} :
+    Dm !! i = Some ((d, α)', Bm, Pm)' → Pm !! k = Some P →
+    depo_stm_tok Dm -∗ lend_itok i k d α P ==∗
+      depo_stm_tok (<[i := ((d, α)', Bm, delete k Pm)']> Dm).
   Proof.
-    move=> ?. iIntros "● l". iMod (own_update_2 with "● l") as "[$$]"; [|done].
-    apply auth_update. rewrite fmap_insert. eapply singleton_local_update.
-    { rewrite lookup_fmap_Some. by eexists _. }
-    apply prod_local_update; [apply prod_local_update|]=>/=; [done| |done].
-    apply: option_local_update. by apply exclusive_local_update.
-  Qed.
-  (** Retrieve for a lender w.r.t. [lend_stm_tok] *)
-  Local Lemma lend_stm_lend_retrieve {Lm i α d P Bm} :
-    Lm !! i = Some (α, (d, P, Lend)', Bm)' →
-    lend_stm_tok Lm -∗ lend_itok i α d P ==∗
-      lend_stm_tok (<[i := (α, (d, P, Dead)', Bm)']> Lm).
-  Proof.
-    move=> ?. iIntros "● l". iMod (own_update_2 with "● l") as "[$_]"; [|done].
+    move=> ??. iIntros "● l". iMod (own_update_2 with "● l") as "[$_]"; [|done].
     apply auth_update. rewrite fmap_insert.
     eapply (singleton_local_update _ _ _ _ _ (_,_,_)).
     { rewrite lookup_fmap_Some. by eexists _. }
-    apply prod_local_update; [apply prod_local_update|]=>/=; [done| |done].
-    apply: option_local_update. by apply exclusive_local_update.
+    apply prod_local_update; [apply prod_local_update|]=>/=; [done..|].
+    rewrite fmap_delete. apply: delete_local_update; last first.
+    { by rewrite lookup_singleton. } exact _.
+  Qed.
+  (** Add lenders w.r.t. [depo_stm_tok] *)
+  Local Lemma depo_stm_lend_add {Dm i d α Bm Pm} Ql :
+    Dm !! i = Some ((d, α)', Bm, Pm)' →
+    depo_stm_tok Dm ==∗
+      depo_stm_tok (<[i := ((d, α)', Bm, map_with Pm Ql)']> Dm) ∗
+      [∗ map] k ↦ Q ∈ map_without Pm Ql, lend_itok i k d α Q.
+  Proof.
+    move=> eq. iIntros "●". iMod (own_update with "●") as "[$ ?]"; last first.
+    { iModIntro. by iApply to_lend_itoks. }
+    rewrite fmap_insert. apply auth_update_alloc, gmap_local_update.
+    move=> i'. case: (decide (i = i'))=> [<-|?]; last first.
+    { rewrite lookup_insert_ne; [|done]. by rewrite lookup_singleton_ne. }
+    rewrite lookup_empty lookup_fmap eq !lookup_insert /=.
+    apply local_update_unital_discrete=> ??. rewrite left_id=> <-. split.
+    { split; [split|]; [done|by apply: gmap_fmap_valid..]. }
+    rewrite -Some_op. f_equiv.
+    split; [split|]=>/=; [by rewrite agree_idemp|by rewrite left_id|].
+    rewrite gmap_op_disj; [|by apply map_disjoint_fmap, map_without_disj].
+    by rewrite -map_fmap_union -map_with_without.
   Qed.
 
-  (** Agreement between [lend_stm_tok] and [bor_itok] *)
-  Local Lemma lend_stm_bor_agree {Lm i j α B} :
-    lend_stm_tok Lm -∗ bor_itok i j α B -∗
-      ⌜∃ C Bm, Lm !! i = Some (α, C, Bm)' ∧ Bm !! j = Some B⌝.
+  (** Agreement between [depo_stm_tok] and [bor_itok] *)
+  Local Lemma depo_stm_bor_agree {Dm i j d α B} :
+    depo_stm_tok Dm -∗ bor_itok i j d α B -∗
+      ⌜∃ Bm Pm, Dm !! i = Some ((d, α)', Bm, Pm)' ∧ Bm !! j = Some B⌝.
   Proof.
     iIntros "● B". iDestruct (own_valid_2 with "● B") as %v. iPureIntro.
-    move: v=> /auth_both_valid_discrete[/singleton_included_l[?[
-      /Some_equiv_eq[?[/lookup_fmap_Some[[?[C Bm]][<-+]]<-]]
-      /Some_included_total/prod_included[/prod_included/=
-        [/to_agree_included/leibniz_equiv_iff ? _]incl]]]_]=> ?.
-    apply singleton_included_exclusive_l in incl; [|apply _| ]; last first.
-    { move=> j'. rewrite lookup_fmap. by case: (Bm !! j'). }
-    move: incl. rewrite lookup_fmap leibniz_equiv_iff fmap_Some.
-    move=> [?[?[?]]]. subst. by eexists _, _.
+    move: v=> /auth_both_valid_discrete[/singleton_included_l[?[++]]_].
+    move=> /Some_equiv_eq[[[??]?][+<-]].
+    move=> /lookup_fmap_Some[[?[??]][[<-<-<-]?]].
+    move=> /Some_included_total/prod_included[/prod_included/=[+ inc]_].
+    move=> /to_agree_included/leibniz_equiv_iff ?.
+    apply singleton_included_exclusive_l in inc;
+      [|exact _|by apply: gmap_fmap_valid]. move: inc.
+    rewrite lookup_fmap leibniz_equiv_iff fmap_Some. move=> [?[?[?]]]. subst.
+    by eexists _, _.
   Qed.
-  (** Update the borrower state w.r.t. [lend_stm_tok] *)
-  Local Lemma lend_stm_bor_stupd {Lm i j α C Bm B B'} :
-    Lm !! i = Some (α, C, Bm)' → Bm !! j = Some B →
-    lend_stm_tok Lm -∗ bor_itok i j α B ==∗
-      lend_stm_tok (<[i := (α, C, <[j := B']> Bm)']> Lm) ∗
-      bor_itok i j α B'.
+  (** Update the borrower state w.r.t. [depo_stm_tok] *)
+  Local Lemma depo_stm_bor_stupd {Dm i j d α Bm Pm B B'} :
+    Dm !! i = Some ((d, α)', Bm, Pm)' → Bm !! j = Some B →
+    depo_stm_tok Dm -∗ bor_itok i j d α B ==∗
+      depo_stm_tok (<[i := ((d, α)', <[j := B']> Bm, Pm)']> Dm) ∗
+      bor_itok i j d α B'.
   Proof.
     move=> ??. iIntros "● B". iMod (own_update_2 with "● B") as "[$$]"; [|done].
     apply auth_update. rewrite fmap_insert. eapply singleton_local_update.
     { rewrite lookup_fmap_Some. by eexists _. }
-    apply prod_local_update; [apply prod_local_update|]=>/=; [done..|].
+    apply prod_local_update; [apply prod_local_update|]=>/=; [done| |done].
     rewrite fmap_insert. apply: singleton_local_update.
     { rewrite lookup_fmap_Some. by eexists _. } by apply exclusive_local_update.
-  Qed.
-  (** Delete the borrower w.r.t. [lend_stm_tok] *)
-  Local Lemma lend_stm_bor_delete {Lm i j α C Bm B} :
-    Lm !! i = Some (α, C, Bm)' → Bm !! j = Some B →
-    lend_stm_tok Lm -∗ bor_itok i j α B ==∗ ∃ Bm',
-      lend_stm_tok (<[i := (α, C, Bm')']> Lm) ∗
-      ⌜∀ Φ : _ → iProp Σ, ([∗ map] B ∈ Bm, Φ B) ⊣⊢ Φ B ∗ [∗ map] B ∈ Bm', Φ B⌝.
-  Proof.
-    move=> ??. iIntros "● B". iExists (delete j Bm).
-    iMod (own_update_2 with "● B") as "[$_]"; last first.
-    { iPureIntro=> ?. by apply big_sepM_delete. }
-    apply auth_update. rewrite fmap_insert.
-    eapply (singleton_local_update _ _ _ _ _ (_,_,_)).
-    { rewrite lookup_fmap_Some. by eexists _. }
-    apply prod_local_update; [apply prod_local_update|]=>/=; [done..|].
-    rewrite fmap_delete.
-    apply: delete_local_update; [|by rewrite lookup_singleton]. apply _.
-  Qed.
-  (** Create a new borrower w.r.t. [lend_stm_tok] *)
-  Local Lemma lend_stm_new_bor {Lm i α C Bm B} :
-    Lm !! i = Some (α, C, Bm)' →
-    lend_stm_tok Lm ==∗ ∃ Bm', lend_stm_tok (<[i := (α, C, Bm')']> Lm) ∗
-      (∃ j, bor_itok i j α B) ∗
-      ⌜∀ Φ : _ → iProp Σ, ([∗ map] B ∈ Bm', Φ B) ⊣⊢ Φ B ∗ [∗ map] B ∈ Bm, Φ B⌝.
-  Proof.
-    move=> Lmi. iIntros "●". iExists (<[fresh (dom Bm) := B]> Bm).
-    iMod (own_update with "●") as "[$ b]"; last first.
-    { iModIntro. iSplit; [by iExists _|]. iPureIntro=> Φ.
-      apply big_sepM_insert, not_elem_of_dom_1, is_fresh. }
-    apply auth_update_alloc. rewrite !fmap_insert.
-    apply gmap_local_update=> j. case: (decide (i = j))=> [<-|?];
-      [|by rewrite !lookup_insert_ne].
-    rewrite !lookup_insert lookup_fmap Lmi lookup_empty.
-    apply local_update_unital_discrete=>/= L _ eq. split.
-    { split; [done|]=>/= ?. rewrite lookup_fmap. by case: (_ !! _). }
-    rewrite left_id in eq. rewrite -eq. apply Some_proper.
-    split; [split|]=>/=; [by rewrite agree_idemp|done|].
-    rewrite fmap_insert. rewrite -insert_singleton_op; [done|].
-    rewrite lookup_fmap. apply fmap_None, not_elem_of_dom_1, is_fresh.
-  Qed.
-  (** Create new borrowers w.r.t. [lend_stm_tok] *)
-  Local Lemma lend_stm_new_bors {Lm i α C Bm Bl} :
-    Lm !! i = Some (α, C, Bm)' →
-    lend_stm_tok Lm ==∗ ∃ Bm', lend_stm_tok (<[i := (α, C, Bm')']> Lm) ∗
-      ([∗ list] B ∈ Bl, ∃ j, bor_itok i j α B) ∗
-      ⌜∀ Φ : _ → iProp Σ,
-        ([∗ map] B ∈ Bm', Φ B) ⊣⊢ ([∗ list] B ∈ Bl, Φ B) ∗ [∗ map] B ∈ Bm, Φ B⌝.
-  Proof.
-    move=> ?. elim: Bl=> /=[|B Bl IH].
-    { iIntros "●". iModIntro. iExists Bm. rewrite insert_id; [|done].
-      iFrame "●". iSplit; [done|]. iPureIntro=> ?. by rewrite left_id. }
-    iIntros "●". iMod (IH with "●") as (Bm') "[●[$ %eq]]".
-    iMod (lend_stm_new_bor with "●") as (Bm'') "[●[$ %eq']]";
-      [by rewrite lookup_insert|].
-    rewrite insert_insert. iModIntro. iExists _. iSplit; [done|].
-    iPureIntro=> ?. by rewrite -assoc -eq.
   Qed.
 End borrow.
 
 (** ** World satisfactions *)
 
 Section borrow.
-  Context `{!borrowGS PROP Σ}.
-  Implicit Type (M : iProp Σ → iProp Σ) (intp : PROP → iProp Σ)
-    (P Q : PROP) (B : bor_st PROP) (Bm : bor_stm PROP) (C : lend_cst PROP).
+  Context `{!borrowGS PROP Σ, !invGS_gen hlc Σ}.
+  Implicit Type (W : iProp Σ) (E : coPset) (intp : PROP → iProp Σ) (P Q : PROP)
+    (D : depo_st PROP) (Dm : depo_stm PROP) (Bm : bor_stm PROP)
+    (Pm : lendm PROP).
 
   (** World satisfaction for a borrower *)
-  Local Definition bor_wsat M intp α d B : iProp Σ :=
+  Local Definition bor_wsat intp d α B : iProp Σ :=
     let '(Q, b)' := B in match b with
     | Clsd => intp Q | Open q => q.[α]
-    | Rebor β => lend_dtok (α ⊓ β) (S d) Q
+    | Rebor β => ∃ d', ⌜d < d'⌝ ∗ lend_dtok d' (α ⊓ β) Q
     end.
 
-  (** World satisfaction for a lender *)
-  Local Definition lend_wsat' M intp α d P Bm : iProp Σ :=
-    ([∗ map] B ∈ Bm, bor_wsat M intp α d B) ∗
-    ([†α] -∗ ([∗ map] '(Q, _)' ∈ Bm, intp Q) -∗ M (intp P)).
-  Local Definition lend_wsat M intp α C Bm : iProp Σ :=
-    let '(d, P, l)' := C in match l with
-    | Lend => lend_wsat' M intp α d P Bm | Dead => [†α]%I
-    end.
+  (** World satisfaction for a deposit *)
+  Local Definition depo_wsat_in W E intp d α Bm Pm : iProp Σ :=
+    ([∗ map] B ∈ Bm, bor_wsat intp d α B) ∗
+    ([†α] -∗ ([∗ map] '(Q, _)' ∈ Bm, intp Q) =[W]{E}=∗ [∗ map] P ∈ Pm, intp P).
+  Local Definition depo_wsat_dead W E intp α Pm : iProp Σ :=
+    [†α] ∗ |=[W]{E}=> [∗ map] P ∈ Pm, intp P.
+  Local Definition depo_wsat W E intp d α Bm Pm : iProp Σ :=
+    depo_wsat_in W E intp d α Bm Pm ∨ depo_wsat_dead W E intp α Pm.
 
   (** World satisfaction for the borrowing machinery *)
-  Local Definition borrow_wsat' M intp g : iProp Σ :=
-    gdepth g ∗ ∃ Lm, lend_stm_tok Lm ∗
-      [∗ map] '(α, C, Bm)' ∈ Lm, lend_wsat M intp α C Bm.
-  Local Definition borrow_wsat_def M intp : iProp Σ :=
-    ∃ g, borrow_wsat' M intp g.
+  Notation borrow_wsat' W E intp Dm :=
+    ([∗ map] '((d, α)', Bm, Pm)' ∈ Dm, depo_wsat W E intp d α Bm Pm)%I.
+  Local Definition borrow_wsat_def W E intp : iProp Σ :=
+    ∃ Dm, depo_stm_tok Dm ∗ borrow_wsat' W E intp Dm.
   Local Definition borrow_wsat_aux : seal borrow_wsat_def.
   Proof. by eexists. Qed.
   Definition borrow_wsat := borrow_wsat_aux.(unseal).
@@ -382,276 +396,425 @@ Section borrow.
   Proof. exact: borrow_wsat_aux.(seal_eq). Qed.
 
   (** Non-expansiveness *)
-  #[export] Instance bor_wsat_ne `{!GenUpd _ M} :
+  #[export] Instance bor_wsat_ne :
     Proper (pointwise_relation _ (⊣⊢) ==> (=) ==> (=) ==> (=) ==> (⊣⊢))
-      (bor_wsat M).
-  Proof. move=> ?? eq ??<-??<-[?[|?|?]]?<-; by rewrite /bor_wsat/= ?eq. Qed.
-  #[export] Instance lend_wsat'_ne `{!GenUpd _ M} :
-    Proper (pointwise_relation _ (⊣⊢) ==> (=) ==> (=) ==> (=) ==> (=) ==> (⊣⊢))
-      (lend_wsat' M).
-  Proof. move=> ?????<-??<-??<-??<-. rewrite /lend_wsat'. repeat f_equiv. Qed.
-  #[export] Instance lend_wsat_ne `{!GenUpd _ M} :
-    Proper (pointwise_relation _ (⊣⊢) ==> (=) ==> (=) ==> (=) ==> (⊣⊢))
-      (lend_wsat M).
+      bor_wsat.
+  Proof. solve_proper. Qed.
+  #[export] Instance depo_wsat_in_ne :
+    Proper ((⊣⊢) ==> (=) ==> pointwise_relation _ (⊣⊢) ==> (=) ==> (=) ==>
+      (=) ==> (=) ==> (⊣⊢)) depo_wsat_in.
+  Proof. solve_proper. Qed.
+  #[export] Instance depo_wsat_dead_ne :
+    Proper ((⊣⊢) ==> (=) ==> pointwise_relation _ (⊣⊢) ==> (=) ==> (=) ==> (⊣⊢))
+      depo_wsat_dead.
+  Proof. solve_proper. Qed.
+  #[export] Instance depo_wsat_ne :
+    Proper ((⊣⊢) ==> (=) ==> pointwise_relation _ (⊣⊢) ==> (=) ==> (=) ==>
+      (=) ==> (=) ==> (⊣⊢)) depo_wsat.
   Proof.
-    move=> ?????<-[?[?[|]]]?<-??<-; rewrite /lend_wsat/=; repeat f_equiv.
+    move=> ?????<-?????<-??<-??<-??<-. rewrite /depo_wsat.
+    f_equiv; solve_proper.
   Qed.
-  #[export] Instance borrow_wsat'_ne `{!GenUpd _ M} :
-    Proper (pointwise_relation _ (⊣⊢) ==> (=) ==> (⊣⊢)) (borrow_wsat' M).
-  Proof. move=> ?????<-. rewrite /borrow_wsat'. repeat f_equiv. Qed.
-  #[export] Instance borrow_wsat_ne `{!GenUpd _ M} :
-    Proper (pointwise_relation _ (⊣⊢) ==> (⊣⊢)) (borrow_wsat M).
+  #[export] Instance borrow_wsat_ne :
+    Proper ((⊣⊢) ==> (=) ==> pointwise_relation _ (⊣⊢) ==> (⊣⊢)) borrow_wsat.
   Proof.
-    move=> ???. rewrite borrow_wsat_unseal /borrow_wsat_def/=. repeat f_equiv.
+    rewrite borrow_wsat_unseal /borrow_wsat_def. move=> ?????<-???.
+    do 6 f_equiv. by apply depo_wsat_ne.
   Qed.
 
-  (** Create a borrower and a lender *)
-  Lemma bor_lend_create' `{!GenUpd _ M} {intp} α P :
-    intp P =[borrow_wsat M intp]=∗ bor_ctok α P ∗ lend_tok α P.
+  (** Create borrowers and lenders with a specific depth *)
+  Local Lemma bor_lend_create_list_dep {W E intp} d α Pl Ql :
+    ([∗ list] P ∈ Pl, intp P) -∗
+    ([†α] -∗ ([∗ list] P ∈ Pl, intp P) =[W]{E}=∗ ([∗ list] Q ∈ Ql, intp Q))
+    =[borrow_wsat W E intp]=∗
+      ([∗ list] P ∈ Pl, bor_ctok α P) ∗ [∗ list] Q ∈ Ql, lend_dtok d α Q.
   Proof.
-    rewrite borrow_wsat_unseal bor_ctok_unseal lend_tok_unseal.
-    iIntros "P [%g[g[%Lm[● Lm]]]]". iMod depth_0 as "d".
-    iMod (lend_stm_create with "●") as (??) "[●[c l]]"; [done..|]. iModIntro.
-    iSplitR "c l d"; last first.
-    { iSplitL "c".
-      { iRight. iExists _. iSplitR; [iApply lft_sincl_refl|]. by iExists _, _. }
-      iExists _. iSplitR; [iApply lft_sincl_refl|]. iExists _. iFrame "d".
-      by iExists _. }
-    iExists _. iFrame "g". iExists _. iFrame "●".
-    iApply (big_sepM_insert_2 with "[P] Lm")=>/=.
-    iSplitL; rewrite big_sepM_singleton /=; by [iLeft|iIntros].
+    rewrite borrow_wsat_unseal bor_ctok_unseal. iIntros "Pl →Ql [%Dm[● Dm]]".
+    iMod (depo_stm_bor_lend_new d α Pl Ql with "●") as (?) "[●[c l]]".
+    iModIntro. rewrite !big_sepM_map_by' big_sepL_fmap.
+    iSplitR "c l"; last first; [iSplitL "c"; iStopProof; do 3 f_equiv;
+      iIntros "[% ?]"; [|by iExists _, _]|].
+    { iRight. iExists _, _, _, _. iSplitR; by [iApply lft_sincl_refl|]. }
+    iExists _. iFrame "●". iApply (big_sepM_insert_2 with "[Pl →Ql] Dm"). iLeft.
+    iSplitL "Pl"; by rewrite !big_sepM_map_by big_sepL_fmap.
   Qed.
-  Lemma bor_lend_create `{!GenUpd _ M} {intp} α P :
-    intp P =[borrow_wsat M intp]=∗ bor_tok α P ∗ lend_tok α P.
-  Proof. rewrite -bor_ctok_tok. by apply bor_lend_create'. Qed.
+  (** Create borrowers and lenders *)
+  Lemma bor_lend_create_list {W E intp} α Pl Ql :
+    ([∗ list] P ∈ Pl, intp P) -∗
+    ([†α] -∗ ([∗ list] P ∈ Pl, intp P) =[W]{E}=∗ ([∗ list] Q ∈ Ql, intp Q))
+    =[borrow_wsat W E intp]=∗
+      ([∗ list] P ∈ Pl, bor_ctok α P) ∗ [∗ list] Q ∈ Ql, lend_tok α Q.
+  Proof.
+    iIntros "Pl →Ql". iMod (bor_lend_create_list_dep 0 with "Pl →Ql") as "[$ ?]".
+    iModIntro. iStopProof. do 3 f_equiv. iIntros "l". rewrite lend_tok_unseal.
+    iExists _. iSplit; [by iApply lft_sincl_refl|]. by iExists _.
+  Qed.
+  (** Simply create a borrower and a lender *)
+  Lemma bor_lend_create {W E intp} α P :
+    intp P =[borrow_wsat W E intp]=∗ bor_ctok α P ∗ lend_tok α P.
+  Proof.
+    iIntros "P". iMod (bor_lend_create_list α [P] [P] with "[P] []")
+      as "[[$_][$_]]"; by [iFrame|iIntros|].
+  Qed.
 
   (** Extend the lender token *)
-  Lemma lend_extend `{!GenUpd _ M} {intp α P} Q :
-    lend_tok α P -∗ (intp P -∗ M (intp Q)) =[borrow_wsat M intp]=∗
-      lend_tok α Q.
+  Lemma lend_extend {W E intp α P} Ql :
+    lend_tok α P -∗ (intp P =[W]{E}=∗ [∗ list] Q ∈ Ql, intp Q)
+      =[borrow_wsat W E intp]=∗ [∗ list] Q ∈ Ql, lend_tok α Q.
   Proof.
     rewrite lend_tok_unseal borrow_wsat_unseal.
-    iIntros "[%α'[#?[%d[d[%i l]]]]] PQ [%g[g[%Lm[● Lm]]]]".
-    iDestruct (lend_stm_lend_agree with "● l") as %[Bm ?].
-    iDestruct (big_sepM_insert_acc with "Lm") as "[L →Lm]"; [done|]=>/=.
-    iMod (lend_stm_lend_extend with "● l") as "[● l]"; [done|]. iModIntro.
-    iSplitR "d l"; last first.
-    { iExists _. iSplitR; [done|]. iExists _. iFrame "d". by iExists _. }
-    iExists _. iFrame "g". iExists _. iFrame "●". iApply "→Lm"=>/=.
-    iDestruct "L" as "[$ →P]"=>/=. iIntros "#† Bm".
-    iMod ("→P" with "† Bm") as "P". iApply ("PQ" with "P").
+    iIntros "[%α'[#?[%d[%i[%k l]]]]] PQ [%Dm[● Dm]]".
+    iDestruct (depo_stm_lend_agree with "● l") as %[Bm[Pm[??]]].
+    iMod (depo_stm_lend_delete with "● l") as "●"; [done..|].
+    iMod (depo_stm_lend_add Ql with "●") as "[● ls]"; [apply lookup_insert|].
+    iModIntro. iSplitR "ls"; last first.
+    { rewrite big_sepM_map_without'. iApply (big_sepL_impl with "ls").
+      iIntros "!> %% ⊑ [% ?]". iExists _. iSplit; [done|]. by iExists _, _, _. }
+    iExists _. iFrame "●". rewrite insert_insert.
+    iDestruct (big_sepM_insert_acc with "Dm") as "[D →Dm]"; [done|]=>/=.
+    iApply "→Dm". iDestruct "D" as "[[Bm →Pm]|[† Pm]]".
+    - iLeft. iFrame "Bm". iIntros "† Bm". iMod ("→Pm" with "† Bm") as "Pm".
+      rewrite big_sepM_map_with.
+      iDestruct (big_sepM_delete with "Pm") as "[? $]"; [done|]. by iApply "PQ".
+    - iRight. iFrame "†". iMod "Pm". rewrite big_sepM_map_with.
+      iDestruct (big_sepM_delete with "Pm") as "[P $]"; [done|]. by iApply "PQ".
   Qed.
 
-  (** [bor_wsat] with the dead lifetime token *)
-  Local Lemma bor_wsat_dead {M intp α d Q b} :
-    [†α] -∗ bor_wsat M intp α d (Q, b)' -∗
-      intp Q ∨ ∃ β, lend_dtok (α ⊓ β) (S d) Q.
+  (** Filter [depo_stm] with a depth *)
+  Local Notation dep_of D := D.1'.1'.
+  Local Notation filter_ge d := (filter (λ iD, d ≤ dep_of iD.2)).
+  Local Notation filter_lt d := (filter (λ iD, dep_of iD.2 < d)).
+  Local Notation filter_eq d := (filter (λ iD, dep_of iD.2 = d)).
+  (** [borrow_wsat'] with deposits under [d] and [α] retrieved *)
+  Local Definition depo_wsat_ret W E intp d' α β Bm Pm : iProp Σ :=
+    if decide (β ⊑ α) then depo_wsat_dead W E intp β Pm
+    else depo_wsat W E intp d' β Bm Pm.
+  Local Definition borrow_wsat_ret W E intp Dm d α : iProp Σ :=
+    ∃ Dm', ⌜filter_lt d Dm' = filter_lt d Dm⌝ ∗ depo_stm_tok Dm' ∗
+      [∗ map] '((d', β)', Bm, Pm)' ∈ filter_ge d Dm',
+        depo_wsat_ret W E intp d' α β Bm Pm.
+
+  (** Retrieve from [borrow_wsat_ret] using [lend_dtok] *)
+  Local Lemma lend_dtok_retrieve {W E intp Dm d d' α β P} : d ≤ d' → β ⊑ α →
+    lend_dtok d' β P =[borrow_wsat_ret W E intp Dm d α ∗ W]{E}=∗ intp P.
   Proof.
-    case b=> [|q|?]; [iIntros; by iLeft| |iIntros; iRight; by iExists _].
-    iIntros "† q". iDestruct (lft_tok_dead with "q †") as "[]".
-  Qed.
-  Local Lemma bor_wsat_list_dead `{!GenUpd _ M} {intp α d Bl} {p q : iProp _} :
-    [†α] -∗ ([∗ list] B ∈ Bl, bor_wsat M intp α d B) -∗
-    (([∗ list] '(Q, _)' ∈ Bl, intp Q) -∗ p -∗ M q) -∗ ∃ Ql,
-      ([∗ list] Q ∈ Ql, ∃ β, lend_dtok (α ⊓ β) (S d) Q) ∗
-      (([∗ list] Q ∈ Ql, intp Q) -∗ p -∗ M q).
-  Proof.
-    move: p. elim: Bl=>/= [|[Q b] Bl IH p].
-    { iIntros. iExists []. by iSplit. } iIntros "#† [B Bl] →q".
-    iDestruct (IH (_∗_)%I with "† Bl [→q]") as (Ql) "[Ql →q]".
-    { iIntros "Bl [Q p]". by iApply ("→q" with "[$Bl Q] p"). }
-    iDestruct (bor_wsat_dead with "† B") as "[Q|l]";
-      [iExists Ql|iExists (Q :: Ql)]=>/=; iFrame "Ql"; [|iFrame "l"];
-      [iIntros "Ql p"|iIntros "[Q Ql] p"]; iApply ("→q" with "Ql [$Q $p]").
-  Qed.
-  (** [lend_wsat'] with the dead lifetime token *)
-  Local Lemma lend_wsat'_dead `{!GenUpd _ M} {intp α d P Bm} :
-    [†α] -∗ lend_wsat' M intp α d P Bm -∗ ∃ Ql,
-      ([∗ list] Q ∈ Ql, ∃ β, lend_dtok (α ⊓ β) (S d) Q) ∗
-      (([∗ list] Q ∈ Ql, intp Q) -∗ M (intp P)).
-  Proof.
-    iIntros "#† [Bl →P]". iDestruct ("→P" with "†") as "→P".
-    rewrite !big_sepM_map_to_list_snd. move: (map_to_list Bm).*2=> Bl.
-    iDestruct (bor_wsat_list_dead (p:=True) with "† Bl [→P]") as (Ql) "[Ql →P]".
-    { iIntros "Bl _".  by iApply ("→P" with "Bl"). }
-    iExists _. iFrame "Ql". iIntros "Ql". by iApply ("→P" with "Ql").
-  Qed.
-  (** Retrieve from the lender token with remaining lender tokens *)
-  Local Lemma lend_pre_retrieve `{!GenUpd _ M} {intp g α d P} :
-    [†α] -∗ lend_dtok α d P =[borrow_wsat' M intp g]=∗ ∃ Ql,
-      ([∗ list] Q ∈ Ql, ∃ β, lend_dtok (α ⊓ β) (S d) Q) ∗
-      (([∗ list] Q ∈ Ql, intp Q) -∗ M (intp P)).
-  Proof.
-    iIntros "#† [d[%i l]] [$[%Lm[● Lm]]]".
-    iDestruct (lend_stm_lend_agree with "● l") as %[Bm ?].
-    iDestruct (big_sepM_insert_acc with "Lm") as "[L →Lm]"; [done|]=>/=.
-    iDestruct (lend_wsat'_dead with "† L") as "$". iExists _.
-    iMod (lend_stm_lend_retrieve with "● l") as "$"; by [|iApply "→Lm"].
-  Qed.
-  (** Retrieve from the lender token,
-    by induction on (the maximum depth minus) the depth *)
-  Local Lemma lend_retrieve' `{!GenUpd _ M} {intp k α d P} :
-    [†α] -∗ lend_dtok α d P =[borrow_wsat' M intp (d + k)]=∗ M (intp P).
-  Proof.
-    move: α d P. elim: k=> [|k IH] α d P; iIntros "#† l";
-      iMod (lend_pre_retrieve with "† l") as (Ql) "[Ql →P]".
-    { case: Ql=> /=[|??]. { by iDestruct ("→P" with "[//]") as "$". }
-      iDestruct "Ql" as "[[%[Sd _]]_]". iIntros "[g _]".
-      iDestruct (depth_bound with "g Sd") as %?. lia. }
-    have -> : d + S k = S d + k by lia. iInduction Ql as [|Q Ql] "IH"=>/=.
-    { by iDestruct ("→P" with "[//]") as "$". }
-    iDestruct "Ql" as "[[%β l] Ql]".
-    iMod (IH with "[†] l") as "Q"; [by rewrite lft_dead_meet_l|].
-    iApply ("IH" with "Ql"). iIntros "Ql". iMod "Q". iApply "→P". iFrame.
-  Qed.
-  Lemma lend_retrieve `{!GenUpd _ M} {intp α P} :
-    [†α] -∗ lend_tok α P =[borrow_wsat M intp]=∗ M (intp P).
-  Proof.
-    rewrite lend_tok_unseal borrow_wsat_unseal.
-    iIntros "#† [%α'[#?[%d[d l]]]] [%g[g W]]".
-    iDestruct (depth_bound with "g d") as %le. move: le=> /Nat.le_sum[?->].
-    iMod (lend_retrieve' with "[†] [$d $l] [$g $W]") as "[W $]";
-      [by iApply lft_sincl_dead_acc|by iExists _].
+    move=> ??. iIntros "[%[% l]] [[%Dm'[%[● Dm']]] W]".
+    iDestruct (depo_stm_lend_agree with "● l") as %[Bm[Pm[eq ?]]].
+    iDestruct (big_sepM_insert_acc with "Dm'") as "[D →Dm']".
+    { rewrite map_filter_lookup_Some. split; [done|simpl; lia]. }
+    rewrite /depo_wsat_ret decide_True; [|done]. iDestruct "D" as "[† Pm]".
+    iMod ("Pm" with "W") as "[$ Pm]".
+    iDestruct (big_sepM_delete with "Pm") as "[$ Pm]"; [done|]=>/=.
+    iMod (depo_stm_lend_delete with "● l") as "●"; [done..|]. iModIntro.
+    iExists _. iFrame "●". iSplit.
+    { iPureIntro. rewrite map_filter_insert_False /=; [|lia].
+      rewrite map_filter_delete_not; [done|]. rewrite eq. move=> ?[<-]/=. lia. }
+    rewrite map_filter_insert_True; [|simpl; lia].
+    iApply "→Dm'". rewrite decide_True; [|done]. by iFrame.
   Qed.
 
-  (** [lend_wsat] with a lifetime token *)
-  Local Lemma lend_wsat_tok {M intp α d Q l Bm q} :
-    q.[α] -∗ lend_wsat M intp α (d, Q, l)' Bm -∗ ⌜l = Lend⌝.
+  (** Retrieve from [bor_wsat] *)
+  Local Lemma bor_wsat_retrieve {W E intp Dm d α β P b} : β ⊑ α →
+    [†β] -∗ bor_wsat intp d β (P, b)'
+      =[borrow_wsat_ret W E intp Dm (S d) α ∗ W]{E}=∗ intp P.
   Proof.
-    iIntros "α †". case: l; by [|iDestruct (lft_tok_dead with "α †") as "[]"].
+    move=> ?. iIntros "† B". case b=> [|q|?]/=; [done|..].
+    { iDestruct (lft_tok_dead with "B †") as "[]". }
+    iDestruct "B" as (??) "l". iApply (lend_dtok_retrieve with "l"); [lia|].
+    etrans; [|done]. apply lft_incl_meet_l.
   Qed.
+  (** Retrieve from [bor_wsat]s *)
+  Local Lemma bor_wsats_retrieve {W E intp Dm d α β Bl} : β ⊑ α →
+    [†β] -∗ ([∗ list] B ∈ Bl, bor_wsat intp d β B)
+      =[borrow_wsat_ret W E intp Dm (S d) α ∗ W]{E}=∗
+      [∗ list] '(P, _)' ∈ Bl, intp P.
+  Proof.
+    move=> ?. elim: Bl; [by iIntros|]=>/= B Bl IH. iIntros "#† [B Bl]".
+    iMod (IH with "† Bl") as "$". by iApply bor_wsat_retrieve.
+  Qed.
+  (** Retrieve from [depo_wsat] *)
+  Local Lemma depo_wsat_retrieve {W E intp Dm d α β Bm Pm} : β ⊑ α →
+    [†β] -∗ depo_wsat W E intp d β Bm Pm
+      =[borrow_wsat_ret W E intp Dm (S d) α ∗ W]{E}=∗
+      depo_wsat_dead W E intp β Pm.
+  Proof.
+    move=> ?. iIntros "#† [[Bl →Pm]|?]"; [|done]. iFrame "†".
+    iDestruct ("→Pm" with "†") as "→Pm". rewrite !big_sepM_map_to_list_snd.
+    move: (map_to_list Bm).*2=> Bl.
+    iMod (bor_wsats_retrieve with "† Bl") as "Bl"; [done..|].
+    by iDestruct ("→Pm" with "Bl") as "$".
+  Qed.
+  (** Retrieve from [depo_wsat]s *)
+  Local Lemma depo_wsats_retrieve {W E intp Dm d α Dl} :
+    [†α] -∗ ([∗ list] '((d', β)', Bm, Pm)' ∈ Dl,
+      if decide (d' = d) then depo_wsat W E intp d' β Bm Pm else emp)
+      =[borrow_wsat_ret W E intp Dm (S d) α ∗ W]{E}=∗
+      [∗ list] '((d', β)', Bm, Pm)' ∈ Dl,
+        if decide (d' = d) then depo_wsat_ret W E intp d' α β Bm Pm else emp.
+  Proof.
+    elim: Dl; [by iIntros|]. move=> [[d' β][??]] Dl IH. iIntros "#† [D Dl]".
+    iMod (IH with "† Dl") as "$". rewrite /depo_wsat_ret.
+    case: (decide (β ⊑ α)); [|done]=> ?. rewrite lft_incl_dead; [|done].
+    case: (decide (d' = d)); [|done]=> ->. by iApply depo_wsat_retrieve.
+  Qed.
+  (** Lemmas for [borrow_wsat_eq_retrieve] *)
+  Local Lemma filter_eq_lt d Dm :
+    filter_eq d Dm = filter_eq d (filter_lt (S d) Dm).
+  Proof.
+    rewrite map_filter_filter. apply map_filter_ext=> ?[[??]?]/=?. lia.
+  Qed.
+  Local Lemma filter_lt_lt d Dm :
+    filter_lt d Dm = filter_lt d (filter_lt (S d) Dm).
+  Proof.
+    rewrite map_filter_filter. apply map_filter_ext=> ?[[??]?]/=?. lia.
+  Qed.
+  (** Retrieve from [borrow_wsat'] on [filter_eq] *)
+  Local Lemma borrow_wsat_eq_retrieve {W E intp Dm d α} :
+    [†α] -∗ borrow_wsat' W E intp (filter_eq d Dm) -∗
+      borrow_wsat_ret W E intp Dm (S d) α =[W]{E}=∗
+      borrow_wsat_ret W E intp Dm d α.
+  Proof.
+    iIntros "† eq ret W". rewrite big_sepM_filter' /= big_sepM_map_to_list_snd.
+    iMod (depo_wsats_retrieve with "† eq [$ret $W]") as "[[ret $] eq]".
+    iModIntro. iDestruct "ret" as (Dm' eq) "[● ret]". iExists _. iFrame "●".
+    rewrite -big_sepM_map_to_list_snd -big_sepM_filter''.
+    rewrite filter_eq_lt (filter_lt_lt d Dm) -!eq -filter_eq_lt -filter_lt_lt.
+    iSplit; [done|].
+    iApply (big_sepM_filter_complement (λ iD, dep_of iD.2 ≠ d)). iStopProof.
+    do 2 f_equiv; rewrite map_filter_filter;
+      apply map_filter_ext=> ?[[??][??]]/= _; lia.
+  Qed.
+  (** Lemma for [borrow_wsat_lt_retrieve] *)
+  Local Lemma borrow_wsat_lt_S_split {W E intp} d Dm :
+    borrow_wsat' W E intp (filter_lt (S d) Dm) ⊣⊢
+      borrow_wsat' W E intp (filter_eq d Dm) ∗
+      borrow_wsat' W E intp (filter_lt d Dm).
+  Proof.
+    rewrite (big_sepM_filter_complement (λ iD, dep_of iD.2 = d)).
+    do 2 f_equiv; rewrite map_filter_filter;
+      apply map_filter_ext=> ?[[??][??]]/= _; lia.
+  Qed.
+  (** Retrieve from [borrow_wsat'] on [filter_lt] *)
+  Local Lemma borrow_wsat_lt_retrieve {W E intp Dm d α} :
+    [†α] -∗ borrow_wsat' W E intp (filter_lt d Dm) -∗
+      borrow_wsat_ret W E intp Dm d α =[W]{E}=∗ borrow_wsat_ret W E intp Dm 0 α.
+  Proof.
+    elim: d; [by iIntros|]=> ? IH. rewrite borrow_wsat_lt_S_split.
+    iIntros "#† [eq lt] ret".
+    iMod (borrow_wsat_eq_retrieve with "† eq ret") as "ret".
+    iApply (IH with "† lt ret").
+  Qed.
+
+  (** Find large enough [d] that empties [filter_ge d Dm] *)
+  Local Lemma filter_ge_empty Dm : ∃ d, filter_ge d Dm = ∅.
+  Proof.
+    induction Dm as [|i[[d' ?]?]?? [d eq]] using map_ind; [by exists 0|].
+    exists (d `max` S d'). rewrite map_filter_insert_False /=; [|lia].
+    rewrite map_filter_delete -(delete_empty i). f_equal.
+    apply (f_equal (filter_ge (S d'))) in eq. move: eq.
+    rewrite map_filter_filter map_filter_empty=> <-.
+    apply map_filter_ext=> ?[[??]?]/=. lia.
+  Qed.
+  (** Retrive using [lend_dtok] *)
+  Lemma lend_retrieve' {W E intp d α P} :
+    [†α] -∗ lend_dtok d α P =[borrow_wsat W E intp ∗ W]{E}=∗ intp P.
+  Proof.
+    rewrite borrow_wsat_unseal. iIntros "† l [[%Dm[● Dm]] W]".
+    case: (filter_ge_empty Dm)=> d' eq.
+    iMod (borrow_wsat_lt_retrieve (d:=d') with "† [Dm] [●] W") as "[W ret]".
+    { iDestruct (big_sepM_filter_complement with "Dm") as "[$ _]". }
+    { iExists _. iFrame "●". rewrite eq. by iSplit. }
+    iMod (lend_dtok_retrieve with "l [$ret $W]") as "[[[%[_[● ?]]] $] $]";
+      [lia|done|]. iModIntro.
+    iExists _. iFrame "●". rewrite map_filter_id; [|lia]. iStopProof.
+    do 2 f_equiv. move=> [[? β][??]]. rewrite /depo_wsat_ret.
+    case: (decide (β ⊑ α))=> ?; [|done]. iIntros. by iRight.
+  Qed.
+  (** Retrive using [lend_tok] *)
+  Lemma lend_retrieve {W E intp α P} :
+    [†α] -∗ lend_tok α P =[borrow_wsat W E intp ∗ W]{E}=∗ intp P.
+  Proof.
+    rewrite lend_tok_unseal. iIntros "† [%α'[⊑[%d l]]]".
+    iDestruct (lft_sincl_dead with "⊑ †") as "†".
+    iApply (lend_retrieve' with "† l").
+  Qed.
+
+  (** [depo_wsat] with a lifetime token *)
+  Local Lemma depo_wsat_tok {W E intp d α Bm Pm q} :
+    q.[α] -∗ depo_wsat W E intp d α Bm Pm -∗
+      q.[α] ∗ depo_wsat_in W E intp d α Bm Pm.
+  Proof.
+    iIntros "α [$|[† _]]"; [done|]. iDestruct (lft_tok_dead with "α †") as "[]".
+  Qed.
+
   (** Update the borrower state to [Open q] *)
-  Local Lemma bor_open_core {M intp i j α P b q} :
-    q.[α] -∗ bor_itok i j α (P, b)' =[borrow_wsat M intp]=∗
-      bor_otok α P q ∗ (∃ d, bor_wsat M intp α d (P, b)').
+  Local Lemma bor_open_core {W E intp i j d α P b q} :
+    q.[α] -∗ bor_itok i j d α (P, b)' =[borrow_wsat W E intp]=∗
+      bor_otok α P q ∗ bor_wsat intp d α (P, b)'.
   Proof.
-    rewrite borrow_wsat_unseal. iIntros "[α α'] b [%g[g[%Lm[● Lm]]]]".
-    iDestruct (lend_stm_bor_agree with "● b") as %[[d[Q l]][Bm[??]]].
-    iDestruct (big_sepM_insert_acc with "Lm") as "[L →Lm]"; [done|]=>/=.
-    iDestruct (lend_wsat_tok with "α L") as %->. iDestruct "L" as "[Bm →Q]"=>/=.
-    iDestruct (big_sepM_insert_acc with "Bm") as "[B →Bm]"; [done|].
-    iMod (lend_stm_bor_stupd with "● b") as "[● o]"; [done..|]. iModIntro.
-    iSplitR "α o B"; last first.
-    { iSplitR "B"; [|by iExists _]. rewrite bor_otok_unseal.
-      iExists α, q. iSplitR; [iApply lft_sincl_refl|]. iSplitR; [by iIntros|].
-      iFrame "α". by iExists _, _. }
-    iExists _. iFrame "g". iExists _. iFrame "●". iApply "→Lm".
-    iSplitR "→Q"=>/=; [by iApply "→Bm"|]. iStopProof.  do 2 f_equiv.
+    rewrite borrow_wsat_unseal. iIntros "[α α'] b [%Dm[● Dm]]".
+    iDestruct (depo_stm_bor_agree with "● b") as %[Bm[Qm[??]]].
+    iDestruct (big_sepM_insert_acc with "Dm") as "[D →Dm]"; [done|].
+    iDestruct (depo_wsat_tok with "α D") as "[α [Bm →Qm]]".
+    iMod (depo_stm_bor_stupd with "● b") as "[● o]"; [done..|].
+    iDestruct (big_sepM_insert_acc with "Bm") as "[$ →Bm]"; [done|]. iModIntro.
+    iSplitR "α o"; last first.
+    { rewrite bor_otok_unseal. iExists _, _, _, _, _.
+      iSplitR; [iApply lft_sincl_refl|]. iSplitR; [by iIntros|]. iFrame. }
+    iExists _. iFrame "●". iApply "→Dm". iLeft.
+    iSplitR "→Qm"=>/=; [by iApply "→Bm"|]. iStopProof. do 2 f_equiv.
     apply bi.equiv_entails_1_1. by apply: big_sepM_insert_override.
   Qed.
   (** Open a closed borrower *)
-  Lemma bor_open' {M intp q α P} :
-    q.[α] -∗ bor_ctok α P =[borrow_wsat M intp]=∗ bor_otok α P q ∗ intp P.
+  Lemma bor_open' {W E intp q α P} :
+    q.[α] -∗ bor_ctok α P =[borrow_wsat W E intp]=∗
+      bor_otok α P q ∗ intp P.
   Proof.
-    rewrite bor_ctok_unseal. iIntros "α [†|[%α'[#?[%i[%j c]]]]]".
+    rewrite bor_ctok_unseal. iIntros "α [†|c]".
     { by iDestruct (lft_tok_dead with "α †") as "[]". }
-    iMod (lft_sincl_tok_acc with "[//] α") as (r) "[α' →α]".
-    iMod (bor_open_core with "α' c") as "[o[%d $]]".
-    iApply (bor_otok_lft with "[//] →α o").
+    iDestruct "c" as (????) "[#⊑ c]".
+    iMod (lft_sincl_tok_acc with "⊑ α") as (r) "[α' →α]".
+    iMod (bor_open_core with "α' c") as "[o $]". iModIntro.
+    iApply (bor_otok_lft with "⊑ →α o").
   Qed.
-  (** Open a borrower, possibly retrieving reborrowing *)
-  Lemma bor_open `{!GenUpd _ M} {intp q α P} :
-    q.[α] -∗ bor_tok α P =[borrow_wsat M intp]=∗ bor_otok α P q ∗ M (intp P).
+  (** Open a borrower *)
+  Lemma bor_open {W E intp q α P} :
+    q.[α] -∗ bor_tok α P =[borrow_wsat W E intp ∗ W]{E}=∗
+      bor_otok α P q ∗ intp P.
   Proof.
-    rewrite bor_tok_unseal. iIntros "α [c|[%α'[#?[%i[%j[%β[† r]]]]]]]".
-    { by iMod (bor_open' with "α c") as "[$$]". }
-    iMod (lft_sincl_tok_acc with "[//] α") as (r') "[α' →α]".
-    iMod (bor_open_core with "α' r") as "[o[%d l]]".
-    iDestruct (bor_otok_lft with "[//] →α o") as "$". rewrite lft_dead_meet_r.
-    iApply (lend_retrieve with "† [l]"). rewrite lend_tok_unseal. iExists _.
-    iSplitR; by [iApply lft_sincl_refl|iExists _].
+    rewrite bor_tok_unseal. iIntros "α [c|r]".
+    { by iMod (bor_open' with "α c"). }
+    iDestruct "r" as (?????) "[#⊑ [#† r]]".
+    iMod (lft_sincl_tok_acc with "⊑ α") as (r) "[α' →α]".
+    iMod (bor_open_core with "α' r") as "[o [%[_ l]]]".
+    iDestruct (bor_otok_lft with "⊑ →α o") as "$".
+    iApply (lend_retrieve' with "[] l").
+    iApply (lft_sincl_dead with "[] †"). iApply lft_sincl_meet_r.
   Qed.
 
-  (** Close a borrower with subdivision *)
-  Lemma bor_subdiv' `{!GenUpd _ M} {intp q α P} Ql :
-    bor_otok α P q -∗ ([∗ list] Q ∈ Ql, intp Q) -∗
-    ([†α] -∗ ([∗ list] Q ∈ Ql, intp Q) -∗ M (intp P)) =[borrow_wsat M intp]=∗
-      q.[α] ∗ ([∗ list] Q ∈ Ql, bor_ctok α Q).
+  (** Open borrow token with the depth and real lifetime explicit *)
+  Local Definition bor_odtok d α α' P q : iProp Σ :=
+    ∃ i j r, α ⊑□ α' ∗ (r.[α'] -∗ q.[α]) ∗ (r/2).[α'] ∗
+      bor_itok i j d α' (P, Open (r/2))'.
+  (** Turn [bor_otok] into [bor_odtok] *)
+  Local Lemma bor_otok_odtok {α P q} :
+    bor_otok α P q ⊢ ∃ d α', α ⊑□ α' ∗ bor_odtok d α α' P q.
   Proof.
-    rewrite bor_otok_unseal borrow_wsat_unseal.
-    iIntros "[%α'[%r[#?[→α[α'[%i[%j o]]]]]]] Ql →P [%g[g[%Lm[● Lm]]]]".
-    iDestruct (lend_stm_bor_agree with "● o") as %[[d[R l]][Bm[??]]].
-    iDestruct (big_sepM_insert_acc with "Lm") as "[L →Lm]"; [done|]=>/=.
-    iDestruct (lend_wsat_tok with "α' L") as %->=>/=.
-    iMod (lend_stm_bor_delete with "● o") as (Bm') "[● %eq]"; [done..|].
-    iMod (lend_stm_new_bors (i:=i) (Bl:=(λ Q,(Q,Clsd)') <$> Ql) with "●") as
-      (Bm'') "[● [bl %eq']]"; [by rewrite lookup_insert|]. iModIntro.
-    rewrite insert_insert big_sepL_fmap. iDestruct "L" as "[Bm →R]".
-    rewrite !eq. iDestruct "Bm" as "[+α' Bm']".
-    iDestruct ("→α" with "[$α' $+α'//]") as "$". iSplitR "bl"; last first.
-    { iApply (big_sepL_impl with "bl"). iIntros "!> %% _ [%j' ?]".
-      rewrite bor_ctok_unseal. iRight. iExists _. iSplit; [done|].
-      by iExists _, _. }
-    iExists _. iFrame "g". iExists _. iFrame "●". iApply "→Lm"=>/=.
-    iSplitL "Bm' Ql"; rewrite !eq' !big_sepL_fmap /=; [by iFrame|].
-    iIntros "#† [Ql Bm]". iMod ("→P" with "[†] Ql") as "P".
-    { by iApply lft_sincl_dead_acc. } iApply ("→R" with "†"). iFrame.
-  Qed.
-  Lemma bor_subdiv `{!GenUpd _ M} {intp q α P} Ql :
-    bor_otok α P q -∗ ([∗ list] Q ∈ Ql, intp Q) -∗
-    ([†α] -∗ ([∗ list] Q ∈ Ql, intp Q) -∗ M (intp P)) =[borrow_wsat M intp]=∗
-      q.[α] ∗ ([∗ list] Q ∈ Ql, bor_tok α Q).
-  Proof.
-    iIntros "o Ql →P". iMod (bor_subdiv' with "o Ql →P") as "[$ Ql]".
-    iModIntro. iStopProof. do 3 f_equiv. exact bor_ctok_tok.
+    rewrite bor_otok_unseal. iDestruct 1 as (α' r ???) "[#⊑ b]". iExists _, _.
+    iFrame "⊑". by iExists _, _, _.
   Qed.
 
+  (** Turn [bor_odtok] to a reborrower using [lend_dtok] *)
+  Local Lemma bor_odtok_reborrow {W E intp d α α' P q β d'} : d < d' →
+    bor_odtok d α α' P q -∗ lend_dtok d' (α' ⊓ β) P =[borrow_wsat W E intp]=∗
+      q.[α] ∗ ([†β] -∗ bor_tok α P).
+  Proof.
+    rewrite borrow_wsat_unseal. iDestruct 1 as (i j r) "[#⊑[→α[α' o]]]".
+    iIntros "[%i'[%k l]] [%Dm [● Dm]]".
+    iDestruct (depo_stm_bor_agree with "● o") as %[Bm[Pm[??]]].
+    iDestruct (big_sepM_insert_acc with "Dm") as "[D →Dm]"; [done|]=>/=.
+    iMod (depo_stm_bor_stupd (B':=(_,Rebor β)') with "● o") as "[● r]";
+      [done..|]. iModIntro.
+    iDestruct (depo_wsat_tok with "α' D") as "[α'[Bm →Pm]]".
+    iDestruct (big_sepM_insert_acc with "Bm") as "[α'2 →Bm]"; [done|].
+    iDestruct ("→α" with "[$α' $α'2]") as "$". iSplitR "r"; last first.
+    { iIntros "†". rewrite bor_tok_unseal. iRight. iExists _, _, _, _, _.
+      by iFrame. }
+    iExists _. iFrame "●". iApply "→Dm". iLeft. iSplitR "→Pm".
+    - iApply "→Bm". iExists _. iSplit; [done|]. by iExists _, _.
+    - iClear "#". iStopProof. do 2 f_equiv=>/=. iIntros "Bm".
+      iApply big_sepM_insert_override; [done| |done]. done.
+  Qed.
+
+  (** Lemma for [bor_merge_subdiv] *)
+  Local Lemma bor_otoks_odtoks_bound {α Pql} :
+    ([∗ list] '(P, q)' ∈ Pql, bor_otok α P q) ⊢ ∃ d β, α ⊑□ β ∗
+      [∗ list] '(P, q)' ∈ Pql, ∃ d' α' β',
+        ⌜d' < d ∧ β = α' ⊓ β'⌝ ∗ bor_odtok d' α α' P q.
+  Proof.
+    elim: Pql=>/=.
+    { iIntros. iExists 0, α. iSplit; [iApply lft_sincl_refl|done]. }
+    move=> [P q] Pql ->. rewrite bor_otok_odtok.
+    iIntros "[[%d[%α'[#⊑ o]]] [%d'[%β[#? big]]]]".
+    iExists (S d `max` d'), (α' ⊓ β).
+    iSplitR; [by iApply lft_sincl_meet_intro|]. iSplitL "o".
+    { iExists _, _, _. iFrame "o". iPureIntro. split; [lia|done]. }
+    iClear "#". iStopProof. do 3 f_equiv.
+    iDestruct 1 as (d'' α'' β' [?->]) "o". iExists _, _, _. iFrame "o".
+    iPureIntro. split; [lia|]. by rewrite assoc [α' ⊓ α'']comm -assoc.
+  Qed.
+  (** Merge and subdivide borrowers *)
+  Lemma bor_merge_subdiv {W E intp α} Pql Ql :
+    ([∗ list] '(P, q)' ∈ Pql, bor_otok α P q) -∗ ([∗ list] Q ∈ Ql, intp Q) -∗
+    ([†α] -∗ ([∗ list] Q ∈ Ql, intp Q) =[W]{E}=∗ [∗ list] P ∈ Pql.*1', intp P)
+      =[borrow_wsat W E intp]=∗
+      ([∗ list] q ∈ Pql.*2', q.[α]) ∗ [∗ list] Q ∈ Ql, bor_ctok α Q.
+  Proof.
+    rewrite bor_otoks_odtoks_bound. iIntros "[%d[%β[#⊑ Pql]]] Ql →P".
+    iMod (bor_lend_create_list_dep d β Ql Pql.*1' with "Ql [→P]")
+      as "[bl ll]"=>/=.
+    { iIntros "† Ql". iDestruct (lft_sincl_dead with "⊑ †") as "†".
+      by iMod ("→P" with "† Ql") as "$". }
+    iSplitR "bl"; last first.
+    { iModIntro. iApply (big_sepL_impl with "bl"). iIntros "!> %% _".
+      by iApply bor_ctok_lft. }
+    iInduction Pql as [|[P q]Pql] "IH"=>/=; [done|].
+    iDestruct "Pql" as "[big Pql]". iDestruct "big" as (???[?->]) "o".
+    iDestruct "ll" as "[l ll]". iMod ("IH" with "Pql ll") as "$".
+    iMod (bor_odtok_reborrow with "o l") as "[$ _]"; [lia|done].
+  Qed.
+  (** Subdivide a borrower *)
+  Lemma bor_subdiv {W E intp α P q} Ql :
+    bor_otok α P q -∗ ([∗ list] Q ∈ Ql, intp Q) -∗
+    ([†α] -∗ ([∗ list] Q ∈ Ql, intp Q) =[W]{E}=∗ intp P)
+      =[borrow_wsat W E intp]=∗ q.[α] ∗ [∗ list] Q ∈ Ql, bor_ctok α Q.
+  Proof.
+    iIntros "o Ql →P".
+    iMod (bor_merge_subdiv [(_,_)'] with "[o] Ql [→P]") as "[[$ _]$]"=>/=;
+      by [iFrame|rewrite bi.sep_emp|].
+  Qed.
   (** Simply close the borrower *)
-  Lemma bor_close' `{!GenUpd _ M} {intp q α P} :
-    bor_otok α P q -∗ intp P =[borrow_wsat M intp]=∗ q.[α] ∗ bor_ctok α P.
+  Lemma bor_close {W E intp q α P} :
+    bor_otok α P q -∗ intp P =[borrow_wsat W E intp]=∗ q.[α] ∗ bor_ctok α P.
   Proof.
-    iIntros "o P". iMod (bor_subdiv' [P] with "o [P] []") as "[$[$_]]"=>/=;
+    iIntros "o P". iMod (bor_subdiv [P] with "o [P] []") as "[$[$_]]"=>/=;
       by [iFrame|iIntros "_[$_]"|].
   Qed.
-  Lemma bor_close `{!GenUpd _ M} {intp q α P} :
-    bor_otok α P q -∗ intp P =[borrow_wsat M intp]=∗ q.[α] ∗ bor_tok α P.
-  Proof. rewrite -bor_ctok_tok. by exact bor_close'. Qed.
 
   (** Reborrow a borrower *)
-  Lemma bor_reborrow' `{!GenUpd _ M} {intp β R r} α :
-    bor_otok β R r -∗ intp R =[borrow_wsat M intp]=∗
-      r.[β] ∗ bor_ctok (α ⊓ β) R ∗ ([†α] -∗ bor_tok β R).
+  Lemma bor_reborrow_o {W E intp α P q} β :
+    bor_otok α P q -∗ intp P =[borrow_wsat W E intp]=∗
+      q.[α] ∗ bor_ctok (α ⊓ β) P ∗ ([†β] -∗ bor_tok α P).
   Proof.
-    rewrite bor_otok_unseal borrow_wsat_unseal.
-    iIntros "[%β'[%s[#?[→β[β'[%i[%j o]]]]]]] R [%g[g[%Lm[● Lm]]]]".
-    iDestruct (lend_stm_bor_agree with "● o") as %[[d[Q l]][Bm[??]]].
-    iDestruct (big_sepM_insert_acc with "Lm") as "[L →Lm]"; [done|]=>/=.
-    iDestruct (lend_wsat_tok with "β' L") as %->.
-    iMod (lend_stm_bor_stupd (B':=(_,Rebor α)') with "● o") as "[● r]";
-      [done..|].
-    iMod (lend_stm_create with "●") as (i' j') "[● [c l]]"; [done..|].
-    iMod (depth_alloc with "g") as (g') "[g d]". iModIntro.
-    iDestruct "L" as "[Bm →Q]"=>/=.
-    iDestruct (big_sepM_insert_acc with "Bm") as "[B →Bm]"; [done|].
-    iDestruct ("→β" with "[$β' $B//]") as "$". iSplitR "c r"; last first.
-    { rewrite bor_tok_unseal bor_ctok_unseal. iSplitL "c"; last first.
-      { iIntros "?". iRight. iExists _. iSplit; [done|]. iExists _, _, _.
-        iFrame. }
-      iRight. iExists _. iSplit; by [iApply lft_sincl_meet_mono_r|iExists _, _].
-    }
-    iExists _. iFrame "g". iExists _. iFrame "●".
-    iApply (big_sepM_insert_2 with "[R]")=>/=.
-    { iSplitL; rewrite big_sepM_singleton /=; by [|iIntros]. }
-    iApply "→Lm". iSplitR "→Q"=>/=.
-    { iApply "→Bm". iFrame "d". rewrite comm. by iExists _. }
-    iClear "#". iStopProof. do 2 f_equiv. apply bi.equiv_entails_1_1.
-    by apply: big_sepM_insert_override.
+    rewrite bor_otok_odtok. iIntros "[%d[%α'[#? o]]] P".
+    iMod (bor_lend_create_list_dep (S d) (α' ⊓ β) [P] [P] with "[P] []")
+      as "[[b _] [l _]]"; [by iFrame|by iIntros|].
+    iMod (bor_odtok_reborrow with "o l") as "[$$]"; [lia|]. iModIntro.
+    iApply (bor_ctok_lft with "[] b"). by iApply lft_sincl_meet_mono_l.
   Qed.
-  Lemma bor_reborrow `{!GenUpd _ M} {intp β R r} α :
-    bor_otok β R r -∗ intp R =[borrow_wsat M intp]=∗
-      r.[β] ∗ bor_tok (α ⊓ β) R ∗ ([†α] -∗ bor_tok β R).
-  Proof. rewrite -bor_ctok_tok. by apply bor_reborrow'. Qed.
+  Lemma bor_reborrow' {W E intp α P q} β :
+    q.[α] -∗ bor_ctok α P =[borrow_wsat W E intp]=∗
+      q.[α] ∗ bor_ctok (α ⊓ β) P ∗ ([†β] -∗ bor_tok α P).
+  Proof.
+    iIntros "α c". iMod (bor_open' with "α c") as "[o P]".
+    by iMod (bor_reborrow_o with "o P").
+  Qed.
+  Lemma bor_reborrow {W E intp α P q} β :
+    q.[α] -∗ bor_tok α P =[borrow_wsat W E intp ∗ W]{E}=∗
+      q.[α] ∗ bor_ctok (α ⊓ β) P ∗ ([†β] -∗ bor_tok α P).
+  Proof.
+    iIntros "α b". iMod (bor_open with "α b") as "[o P]".
+    by iMod (bor_reborrow_o with "o P").
+  Qed.
 End borrow.
 
 (** Allocate [borrow_wsat] *)
-Lemma borrow_wsat_alloc `{!borrowGpreS PROP Σ} :
-  ⊢ |==> ∃ _ : borrowGS PROP Σ, ∀ M intp, borrow_wsat M intp.
+Lemma borrow_wsat_alloc `{!borrowGpreS PROP Σ, !invGS_gen hlc Σ} :
+  ⊢ |==> ∃ _ : borrowGS PROP Σ, ∀ W E intp, borrow_wsat W E intp.
 Proof.
-  iMod (own_alloc (● (MaxNat 0))) as (γ) "g"; [by apply auth_auth_valid|].
-  iMod (own_alloc (● (∅ : gmapR _ _))) as (γ') "●";
-    [by apply auth_auth_valid|]. iModIntro.
-  iExists (BorrowGS _ _ _ _ _ γ γ'). iIntros (M intp).
-  rewrite borrow_wsat_unseal. iExists _. iFrame "g". iExists ∅. by iFrame.
+  iMod (own_alloc (● (∅ : gmapR _ _))) as (γ) "●"; [by apply auth_auth_valid|].
+  iModIntro. iExists (BorrowGS _ _ _ _ γ). iIntros (???).
+  rewrite borrow_wsat_unseal. iExists ∅. by iFrame.
 Qed.
 
 (** ** Fractured borrowing *)
@@ -674,12 +837,12 @@ Definition fborrowΣ PROP : gFunctors := ghost_mapΣ positive (fbor_st PROP).
 Proof. solve_inG. Qed.
 
 Section fborrow.
-  Context `{!fborrowGS PROP Σ, !borrowGS PROP Σ}.
+  Context `{!fborrowGS PROP Σ, !borrowGS PROP Σ, !invGS_gen hlc Σ}.
   Implicit Type (Φ : Qp → PROP) (F : fbor_stm PROP).
 
   (** Fractional borrower token *)
   Definition fbor_tok_def α Φ : iProp Σ :=
-    ∃ α', α ⊑s α' ∗ ∃ i, i ↪[fborrow_name]□ (α', Φ)'.
+    ∃ α', α ⊑□ α' ∗ ∃ i, i ↪[fborrow_name]□ (α', Φ)'.
   Lemma fbor_tok_aux : seal (@fbor_tok_def). Proof. by eexists. Qed.
   Definition fbor_tok := fbor_tok_aux.(unseal).
   Lemma fbor_tok_unseal : @fbor_tok = @fbor_tok_def.
@@ -687,10 +850,10 @@ Section fborrow.
 
   (** [fbor_tok] is persistent *)
   #[export] Instance fbor_tok_persistent α Φ : Persistent (fbor_tok α Φ).
-  Proof. rewrite fbor_tok_unseal. apply _. Qed.
+  Proof. rewrite fbor_tok_unseal. exact _. Qed.
 
   (** Modify the lifetime of [fbor_tok] *)
-  Lemma fbor_tok_lft {α α' Φ} : α' ⊑s α -∗ fbor_tok α Φ -∗ fbor_tok α' Φ.
+  Lemma fbor_tok_lft {α α' Φ} : α' ⊑□ α -∗ fbor_tok α Φ -∗ fbor_tok α' Φ.
   Proof.
     rewrite fbor_tok_unseal. iIntros "#? [%α''[#? f]]". iExists _. iFrame "f".
     by iApply lft_sincl_trans.
@@ -699,82 +862,44 @@ Section fborrow.
   (** World satisfaction for the fractional borrowing machinery *)
   Definition fborrow_wsat_def : iProp Σ :=
     ∃ F, ghost_map_auth fborrow_name 1 F ∗
-      ([∗ map] '(α, Φ)' ∈ F, ∃ q, bor_ctok α (Φ q)).
+      ([∗ map] '(α, Φ)' ∈ F, ∃ q, bor_tok α (Φ q)).
   Lemma fborrow_wsat_aux : seal fborrow_wsat_def. Proof. by eexists. Qed.
   Definition fborrow_wsat := fborrow_wsat_aux.(unseal).
   Lemma fborrow_wsat_unseal : fborrow_wsat = fborrow_wsat_def.
   Proof. exact: fborrow_wsat_aux.(seal_eq). Qed.
 
-  (** Turn [bor_ctok] into [fbor_tok] *)
-  Lemma bor_fbor' {α Φ q} : bor_ctok α (Φ q) =[fborrow_wsat]=∗ fbor_tok α Φ.
+  (** Turn [bor_tok] into [fbor_tok] *)
+  Lemma bor_fbor {α Φ q} : bor_tok α (Φ q) =[fborrow_wsat]=∗ fbor_tok α Φ.
   Proof.
-    rewrite fborrow_wsat_unseal. iIntros "c [%F[● F]]".
+    rewrite fborrow_wsat_unseal. iIntros "b [%F[● F]]".
     iMod (ghost_map_insert_persist with "●") as "[● i]";
       [apply not_elem_of_dom_1, is_fresh|]. iModIntro.
-    iDestruct (big_sepM_insert_2 _ _ _ (_,_)' with "[c] F") as "F";
+    iDestruct (big_sepM_insert_2 _ _ _ (_,_)' with "[b] F") as "F";
       [by iExists q|].
     iSplitR "i"; [iExists _; iFrame|]. rewrite fbor_tok_unseal. iExists _.
     iSplit; by [iApply lft_sincl_refl|iExists _].
   Qed.
-  Lemma bor_fbor `{!GenUpd _ M} {intp α Φ q r} :
-    bor_otok α (Φ q) r -∗ intp (Φ q) =[fborrow_wsat ∗ borrow_wsat M intp]=∗
-      fbor_tok α Φ ∗ r.[α].
-  Proof.
-    iIntros "o Φ". iMod (bor_close' with "o Φ") as "[$ c]".
-    by iMod (bor_fbor' with "c") as "$".
-  Qed.
-
-  (** Get [fbor_tok] from borrow subdivision *)
-  Lemma bor_subdivf' `{!GenUpd _ M} {intp q α P} Ql Φrl :
-    bor_otok α P q -∗ ([∗ list] Q ∈ Ql, intp Q) -∗
-    ([∗ list] '(Φ, r)' ∈ Φrl, intp (Φ r)) -∗
-    ([†α] -∗ ([∗ list] Q ∈ Ql, intp Q) -∗
-      ([∗ list] '(Φ, r)' ∈ Φrl, intp (Φ r)) -∗ M (intp P))
-      =[fborrow_wsat ∗ borrow_wsat M intp]=∗
-      q.[α] ∗ ([∗ list] Q ∈ Ql, bor_ctok α Q) ∗
-      [∗ list] '(Φ, r)' ∈ Φrl, fbor_tok α Φ.
-  Proof.
-    iIntros "o Ql Φrl →P".
-    iMod (bor_subdiv' (Ql ++ ((λ '(Φ, r)', Φ r) <$> Φrl))
-      with "o [$Ql Φrl] [→P]") as "[$[$ cl]]"; [by rewrite big_sepL_fmap| |].
-    { iIntros "† [Ql Φrl]". rewrite big_sepL_fmap.
-      iApply ("→P" with "† Ql Φrl"). }
-    iStopProof. elim: Φrl=> [|[Φ r] Φrl IH]/=; [by iIntros|].
-    iIntros "[b bl]". iMod (IH with "bl") as "$". by iMod (bor_fbor' with "b").
-  Qed.
-  Lemma bor_subdivf `{!GenUpd _ M} {intp q α P} Ql Φrl :
-    bor_otok α P q -∗ ([∗ list] Q ∈ Ql, intp Q) -∗
-    ([∗ list] '(Φ, r)' ∈ Φrl, intp (Φ r)) -∗
-    ([†α] -∗ ([∗ list] Q ∈ Ql, intp Q) -∗
-      ([∗ list] '(Φ, r)' ∈ Φrl, intp (Φ r)) -∗ M (intp P))
-      =[fborrow_wsat ∗ borrow_wsat M intp]=∗
-      q.[α] ∗ ([∗ list] Q ∈ Ql, bor_tok α Q) ∗
-      [∗ list] '(Φ, r)' ∈ Φrl, fbor_tok α Φ.
-  Proof.
-    iIntros "o Ql Φrl →P". iMod (bor_subdivf' with "o Ql Φrl →P") as "[$[? $]]".
-    iModIntro. iStopProof. do 3 f_equiv. exact bor_ctok_tok.
-  Qed.
 
   (** Open [fbor_tok] *)
-  Lemma fbor_open `{!GenUpd _ M} {intp α q} `(Fractional _ (intp ∘ Φ)) :
-    q.[α] -∗ fbor_tok α Φ =[fborrow_wsat ∗ borrow_wsat M intp]=∗
+  Lemma fbor_open {W E intp α q} `(!Fractional (intp ∘ Φ)) :
+    q.[α] -∗ fbor_tok α Φ =[fborrow_wsat ∗ borrow_wsat W E intp ∗ W]{E}=∗
       ∃ r, bor_otok α (Φ r) q ∗ intp (Φ r).
   Proof.
     rewrite fbor_tok_unseal fborrow_wsat_unseal.
-    iIntros "α [%α'[#?[%i i]]] [[%F[● F]]W]".
+    iIntros "α [%α'[#?[%i i]]] [[%F[● F]] BW]".
     iMod (lft_sincl_tok_acc with "[//] α") as (s) "[α' →α]".
     iDestruct (ghost_map_lookup with "● i") as %?.
-    iDestruct (big_sepM_lookup_acc with "F") as "[[%r c]→F]"; [done|]=>/=.
-    iMod (bor_open' with "α' c W") as "[W[o Φ]]".
+    iDestruct (big_sepM_lookup_acc with "F") as "[[%r b]→F]"; [done|]=>/=.
+    iMod (bor_open with "α' b BW") as "[[B $] [o Φ]]".
     have eq : intp (Φ r) ⊣⊢ intp (Φ (r/2)%Qp) ∗ intp (Φ (r/2)%Qp).
     { by erewrite fractional_half; [|apply: fractional_as_fractional]. }
     rewrite eq. iDestruct "Φ" as "[Φ Φ']".
-    iMod (bor_subdiv' [_;_] with "o [Φ Φ'] [] W") as "[W[α'[c[c' _]]]]".
+    iMod (bor_subdiv [_;_] with "o [Φ Φ'] [] B") as "[B [α'[c[c' _]]]]".
     { by iFrame. } { rewrite eq. by iIntros "_ [$[$ _]]". }
-    iMod (bor_open' with "α' c' W") as "[$[o Φ]]". iModIntro.
+    iMod (bor_open' with "α' c' B") as "[$ [o Φ]]". iModIntro.
     iDestruct (bor_otok_lft with "[//] →α o") as "o".
     iSplitR "o Φ"; [|iExists _; by iFrame]. iExists _. iFrame "●". iApply "→F".
-    by iExists _.
+    rewrite bor_ctok_tok. by iExists _.
   Qed.
 End fborrow.
 
